src/Lean/Elab/Tactic/Try.lean
@@ -599,21 +599,29 @@ private def mkSimpleTacStx : CoreM (TSyntax `tactic) :=
 /-! Function induction generators -/
 
 open Try.Collector in
-private def mkFunIndStx (expr : Expr) (cont : TSyntax `tactic) : MetaM (Array (TSyntax `tactic)) := do
+private def mkFunIndStx (uniques : NameSet) (expr : Expr) (cont : TSyntax `tactic) : MetaM (Array (TSyntax `tactic)) := do
   let isAccessible ← isExprAccessible expr
   withExposedNames do
-    let stx ← PrettyPrinter.delab expr
+    let fn := expr.getAppFn.constName!
+    let stx ←
+      -- If it is unambigous, use `fun_induction foo` without arguments
+      if uniques.contains fn then
+        let t : Term ← toIdent fn
+        pure t
+      else
+        PrettyPrinter.delab expr
     let tac₁ ← `(tactic| fun_induction $stx <;> $cont)
     -- if expr has no inaccessible names, use as is
     if isAccessible then
       return #[tac₁]
     else
-      -- if it does, still try without, in case they are all implicit
+      -- if it has inaccessible names, still try without, in case they are all implicit
       let tac₂ ← `(tactic| (expose_names; $tac₁))
       return #[tac₁, tac₂]
 
 private def mkAllFunIndStx (info : Try.Info) (cont : TSyntax `tactic) : MetaM (TSyntax `tactic) := do
-  let tacs ← info.funIndCandidates.calls.flatMapM (mkFunIndStx · cont)
+  let uniques := info.funIndCandidates.uniques
+  let tacs ← info.funIndCandidates.calls.flatMapM (mkFunIndStx uniques · cont)
   mkFirstStx tacs
 
 /-! Main code -/
